Define what each actor trace must look like to be compatible with reduction

ironfleet/src/Dafny/Distributed/Concur/EventHandler.i.dfy
@@ -1,9 +1,52 @@
 include "DistributedSystem.i.dfy"
-include "Movers.i.dfy"
+include "Reduction.i.dfy"
 
 module EventHandlerModule {
     import opened DistributedSystemModule
-    import opened MoversModule
+    import opened ReductionModule
+
+    predicate IOActionsCompatibleWithReductionUsingPivot(ios:seq<IOAction>, pivot:int)
+    {
+           0 <= pivot < |ios|
+        && (forall i :: 0 <= i < pivot ==> IOActionIsRightMover(ios[i]))
+        && (forall i :: pivot < i < |ios| ==> IOActionIsLeftMover(ios[i]))
+    }
+
+    predicate IOActionsCompatibleWithReduction(ios:seq<IOAction>)
+    {
+        |ios| == 0 || exists pivot :: IOActionsCompatibleWithReductionUsingPivot(ios, pivot)
+    }
+
+    lemma lemma_IfIOActionsCompatibleWithReductionAndOneIsntRightMoverThenRestAreLeftMovers(ios:seq<IOAction>, i:int, j:int)
+        requires 0 <= i < j < |ios|;
+        requires IOActionsCompatibleWithReduction(ios);
+        requires !IOActionIsRightMover(ios[i]);
+        ensures  IOActionIsLeftMover(ios[j]);
+        decreases j;
+    {
+        var pivot :| IOActionsCompatibleWithReductionUsingPivot(ios, pivot);
+        assert !(i < pivot);
+        assert j > pivot;
+    }
+
+    lemma lemma_IfIOActionsCompatibleWithReductionThenSuffixIs(ios:seq<IOAction>)
+        requires |ios| > 0;
+        requires IOActionsCompatibleWithReduction(ios);
+        ensures  IOActionsCompatibleWithReduction(ios[1..]);
+    {
+        var ios' := ios[1..];
+        if |ios'| == 0 {
+            return;
+        }
+        
+        var pivot :| IOActionsCompatibleWithReductionUsingPivot(ios, pivot);
+        if pivot == 0 {
+            assert IOActionsCompatibleWithReductionUsingPivot(ios', 0);
+        }
+        else {
+            assert IOActionsCompatibleWithReductionUsingPivot(ios', pivot-1);
+        }
+    }
 
     function CombineIOActions(ios:seq<IOAction>) : seq<IOAction>
     {
