ironfleet/src/Dafny/Distributed/Concur/Movers.i.dfy
@@ -34,49 +34,6 @@ module MoversModule {
         entry.EntryAction? ==> ActionIsLeftMover(entry.action)
     }
 
-    predicate IOActionsCompatibleWithReductionUsingPivot(ios:seq<IOAction>, pivot:int)
-    {
-           0 <= pivot < |ios|
-        && (forall i :: 0 <= i < pivot ==> IOActionIsRightMover(ios[i]))
-        && (forall i :: pivot < i < |ios| ==> IOActionIsLeftMover(ios[i]))
-    }
-
-    predicate IOActionsCompatibleWithReduction(ios:seq<IOAction>)
-    {
-        |ios| == 0 || exists pivot :: IOActionsCompatibleWithReductionUsingPivot(ios, pivot)
-    }
-
-    lemma lemma_IfIOActionsCompatibleWithReductionAndOneIsntRightMoverThenRestAreLeftMovers(ios:seq<IOAction>, i:int, j:int)
-        requires 0 <= i < j < |ios|;
-        requires IOActionsCompatibleWithReduction(ios);
-        requires !IOActionIsRightMover(ios[i]);
-        ensures  IOActionIsLeftMover(ios[j]);
-        decreases j;
-    {
-        var pivot :| IOActionsCompatibleWithReductionUsingPivot(ios, pivot);
-        assert !(i < pivot);
-        assert j > pivot;
-    }
-
-    lemma lemma_IfIOActionsCompatibleWithReductionThenSuffixIs(ios:seq<IOAction>)
-        requires |ios| > 0;
-        requires IOActionsCompatibleWithReduction(ios);
-        ensures  IOActionsCompatibleWithReduction(ios[1..]);
-    {
-        var ios' := ios[1..];
-        if |ios'| == 0 {
-            return;
-        }
-        
-        var pivot :| IOActionsCompatibleWithReductionUsingPivot(ios, pivot);
-        if pivot == 0 {
-            assert IOActionsCompatibleWithReductionUsingPivot(ios', 0);
-        }
-        else {
-            assert IOActionsCompatibleWithReductionUsingPivot(ios', pivot-1);
-        }
-    }
-
     lemma lemma_MoverCommutativityForIOActions(
         actor1:Actor,
         actor2:Actor,
